add if tactic

Forward.v
@@ -29,3 +29,52 @@ Proof.
     + auto.
     + apply int_aeval_sound. auto.
 Qed.
+
+(* TODO placeholder *)
+Definition forward_cond (s : assertion) (b : bexp) : assertion.
+Admitted.
+
+Lemma forward_cond_valid (s : assertion) (b : bexp) (res : assertion) :
+  res = forward_cond s b ->
+  (forall st : state, st |= s -> beval st b = true -> st |= res).
+Admitted.
+
+Definition forward_cond_true (s : assertion) (b : bexp) : assertion :=
+  forward_cond s b.
+
+Lemma forward_cond_true_valid (s : assertion) (b : bexp) (res : assertion) :
+  res = forward_cond_true s b ->
+  (forall st : state, st |= s -> beval st b = true -> st |= res).
+Proof.
+  apply forward_cond_valid.
+Qed.
+
+Definition forward_cond_false (s : assertion) (b : bexp) : assertion :=
+  forward_cond s (BNot b).
+
+Lemma forward_cond_false_valid (s : assertion) (b : bexp) (res : assertion) :
+  res = forward_cond_false s b ->
+  (forall st : state, st |= s -> beval st b = false -> st |= res).
+Proof.
+  intros. assert (beval st (BNot b) = true). {
+    simpl. rewrite H1.  auto.
+  }
+  eapply forward_cond_valid with (b := (BNot b)); eauto.
+Qed.
+
+Lemma forward_if (s : assertion) (b : bexp) (A1 A2 : annotation) (s' : assertion) :
+  step_valid A1 ->
+  step_valid A2 ->
+  (forall st : state, st |= s -> beval st b = true -> st |= precondition A1) ->
+  (forall st : state, st |= s -> beval st b = false -> st |= precondition A2) ->
+  forall (res : assertion),
+  res = join s' (join (postcondition A1) (postcondition A2)) ->
+  step_valid' s (AIf b A1 A2 res).
+Proof.
+  intros. apply SVIf; auto.
+  all : subst; eapply assertion_in_assertion_trans; apply le_assertion_in_assertion;
+  [ | eapply proj2; eapply join_sound].
+  - eapply proj1; eapply join_sound.
+  - eapply proj2; eapply join_sound.
+Qed.
+
